work on adding Disk

concurrency/framework/DiskSSM.s.dfy
@@ -1,8 +1,10 @@
 include "PCM.s.dfy"
 include "StateMachines.s.dfy"
+include "../../lib/Lang/NativeTypes.s.dfy"
 
 abstract module DiskSSM(IOIfc: InputOutputIfc) {
   import opened RequestIds
+  import opened NativeTypes
 
   type M(!new)
 
@@ -16,6 +18,12 @@ abstract module DiskSSM(IOIfc: InputOutputIfc) {
   // there are only a finite number of them (i.e., it is always possible to find
   // a free one).
   function request_ids_in_use(m: M) : set<RequestId>
+
+  function DiskWriteReq(disk_addr: int, data: seq<byte>) : M
+  function DiskWriteResp(disk_addr: int) : M
+
+  function DiskReadReq(disk_addr: int) : M
+  function DiskReadResp(disk_addr: int, data: seq<byte>) : M
 
   predicate Init(s: M)
   predicate Internal(shard: M, shard': M)
@@ -49,6 +57,14 @@ abstract module DiskSSM(IOIfc: InputOutputIfc) {
   requires Inv(whole)
   requires ConsumeStub(whole, whole', rid, output)
   ensures Inv(whole')
+
+  lemma ProcessReadPreservesInv(disk_addr: int, data: seq<byte>, rest: M)
+  requires Inv(dot(DiskReadReq(disk_addr), rest))
+  ensures Inv(dot(DiskReadResp(disk_addr, data), rest))
+
+  lemma ProcessWritePreservesInv(disk_addr: int, data: seq<byte>, rest: M)
+  requires Inv(dot(DiskWriteReq(disk_addr, data), rest))
+  ensures Inv(dot(DiskWriteResp(disk_addr), rest))
 
   lemma dot_unit(x: M)
   ensures dot(x, unit()) == x
@@ -93,6 +109,7 @@ module TicketStubStateMachine(IOIfc: InputOutputIfc, ssm: TicketStubSSM(IOIfc))
   }
 }
 
+/*
 module Obligations(
     IOIfc: InputOutputIfc,
     ssm: TicketStubSSM(IOIfc),
@@ -104,3 +121,4 @@ module Obligations(
        )
   )
 { }
+*/
