concurrency/framework/AsyncDisk.s.dfy
@@ -1,0 +1,202 @@
+include "../../lib/Lang/NativeTypes.s.dfy"
+include "StateMachines.s.dfy"
+
+module DiskIfc refines Ifc {
+  import opened NativeTypes
+  import opened RequestIds
+
+  datatype ReqRead = ReqRead(addr: uint64, len: uint64)
+  datatype ReqWrite = ReqWrite(addr: uint64, bytes: seq<byte>)
+  datatype RespRead = RespRead(addr: uint64, bytes: seq<byte>)
+  datatype RespWrite = RespWrite(addr: uint64, len: uint64)
+
+  datatype DiskOp =
+    | ReqReadOp(id: RequestId, reqRead: ReqRead)
+    | ReqWriteOp(id: RequestId, reqWrite: ReqWrite)
+    | RespReadOp(id: RequestId, respRead: RespRead)
+    | RespWriteOp(id: RequestId, respWrite: RespWrite)
+    | NoDiskOp
+
+  type Op = DiskOp
+}
+
+module AsyncDisk refines StateMachine(DiskIfc) {
+  import opened NativeTypes
+
+  import opened DiskIfc
+
+  type ReqId = uint64
+
+  datatype ReqRead = ReqRead(addr: uint64, len: uint64)
+  datatype ReqWrite = ReqWrite(addr: uint64, bytes: seq<byte>)
+  datatype RespRead = RespRead(addr: uint64, bytes: seq<byte>)
+  datatype RespWrite = RespWrite(addr: uint64, len: uint64)
+
+  datatype DiskOp =
+    | ReqReadOp(id: ReqId, reqRead: ReqRead)
+    | ReqWriteOp(id: ReqId, reqWrite: ReqWrite)
+    | RespReadOp(id: ReqId, respRead: RespRead)
+    | RespWriteOp(id: ReqId, respWrite: RespWrite)
+    | NoDiskOp
+
+  datatype Variables = Variables(
+    // Queue of requests and responses:
+    reqReads: map<ReqId, ReqRead>,
+    reqWrites: map<ReqId, ReqWrite>,
+    respReads: map<ReqId, RespRead>,
+    respWrites: map<ReqId, RespWrite>,
+
+    // The disk:
+    contents: seq<byte>
+  )
+
+  predicate Init(s: Variables)
+  {
+    && s.reqReads == map[]
+    && s.reqWrites == map[]
+    && s.respReads == map[]
+    && s.respWrites == map[]
+  }
+
+  datatype Step =
+    | RecvReadStep
+    | RecvWriteStep
+    | AckReadStep
+    | AckWriteStep
+    | StutterStep
+
+  predicate RecvRead(s: Variables, s': Variables, dop: DiskOp)
+  {
+    && dop.ReqReadOp?
+    && dop.id !in s.reqReads
+    && dop.id !in s.respReads
+    && s' == s.(reqReads := s.reqReads[dop.id := dop.reqRead])
+  }
+
+  predicate RecvWrite(s: Variables, s': Variables, dop: DiskOp)
+  {
+    && dop.ReqWriteOp?
+    && dop.id !in s.reqWrites
+    && dop.id !in s.respWrites
+    && s' == s.(reqWrites := s.reqWrites[dop.id := dop.reqWrite])
+  }
+
+  predicate AckRead(s: Variables, s': Variables, dop: DiskOp)
+  {
+    && dop.RespReadOp?
+    && dop.id in s.respReads
+    && s.respReads[dop.id] == dop.respRead
+    && s' == s.(respReads := s.respReads - {dop.id})
+  }
+
+  predicate AckWrite(s: Variables, s': Variables, dop: DiskOp)
+  {
+    && dop.RespWriteOp?
+    && dop.id in s.respWrites
+    && s.respWrites[dop.id] == dop.respWrite
+    && s' == s.(respWrites := s.respWrites - {dop.id})
+  }
+
+  predicate Stutter(s: Variables, s': Variables, dop: DiskOp)
+  {
+    && dop.NoDiskOp?
+    && s' == s
+  }
+
+  predicate NextStep(s: Variables, s': Variables, dop: DiskOp, step: Step) {
+    match step {
+      case RecvReadStep => RecvRead(s, s', dop)
+      case RecvWriteStep => RecvWrite(s, s', dop)
+      case AckReadStep => AckRead(s, s', dop)
+      case AckWriteStep => AckWrite(s, s', dop)
+      case StutterStep => Stutter(s, s', dop)
+    }
+  }
+
+  predicate Next(s: Variables, s': Variables, op: ifc.Op) {
+    exists step :: NextStep(s, s', op, step)
+  }
+
+  datatype InternalStep =
+    | ProcessReadStep(id: ReqId)
+    | ProcessWriteStep(id: ReqId)
+    | HavocConflictingWritesStep(id: ReqId, id': ReqId)
+    | HavocConflictingWriteReadStep(id: ReqId, id': ReqId)
+
+  predicate ProcessRead(s: Variables, s': Variables, id: ReqId)
+  {
+    && id in s.reqReads
+    && var req := s.reqReads[id];
+    && 0 <= req.addr as int <= req.addr as int + req.len as int <= |s.contents|
+    && s' == s.(reqReads := MapRemove1(s.reqReads, id))
+              .(respReads := s.respReads[id := RespRead(req.addr, s.contents[req.addr .. req.addr as int + req.len as int])])
+  }
+
+  function {:opaque} splice(bytes: seq<byte>, start: int, ins: seq<byte>) : seq<byte>
+  requires 0 <= start
+  requires start + |ins| <= |bytes|
+  {
+    bytes[.. start] + ins + bytes[start + |ins| ..]
+  }
+
+  predicate ProcessWrite(s: Variables, s': Variables, id: ReqId)
+  {
+    && id in s.reqWrites
+    && var req := s.reqWrites[id];
+    && 0 <= req.addr
+    && |req.bytes| < 0x1_0000_0000_0000_0000
+    && req.addr as int + |req.bytes| <= |s.contents|
+    && s' == s.(reqWrites := MapRemove1(s.reqWrites, id))
+              .(respWrites := s.respWrites[id := RespWrite(req.addr, |req.bytes| as uint64)])
+              .(contents := splice(s.contents, req.addr as int, req.bytes))
+  }
+
+  // We assume the disk makes ABSOLUTELY NO GUARANTEES about what happens
+  // when there are conflicting reads or writes.
+
+  predicate overlap(start: int, len: int, start': int, len': int)
+  {
+    && start + len > start'
+    && start' + len' > start
+  }
+
+  predicate HavocConflictingWrites(s: Variables, s': Variables, id: ReqId, id': ReqId)
+  {
+    && id != id'
+    && id in s.reqWrites
+    && id' in s.reqWrites
+    && overlap(
+        s.reqWrites[id].addr as int, |s.reqWrites[id].bytes|,
+        s.reqWrites[id'].addr as int, |s.reqWrites[id'].bytes|)
+  }
+
+  predicate HavocConflictingWriteRead(s: Variables, s': Variables, id: ReqId, id': ReqId)
+  {
+    && id in s.reqWrites
+    && id' in s.reqReads
+    && overlap(
+        s.reqWrites[id].addr as int, |s.reqWrites[id].bytes|,
+        s.reqReads[id'].addr as int, s.reqReads[id'].len as int)
+  }
+
+  predicate NextInternalStep(s: Variables, s': Variables, step: InternalStep)
+  {
+    match step {
+      //case ProcessReadStep(id) => ProcessRead(s, s', id)
+      case ProcessReadFailureStep(id, fakeContents) => ProcessReadFailure(s, s', id, fakeContents)
+      case ProcessWriteStep(id) => ProcessWrite(s, s', id)
+      case HavocConflictingWritesStep(id, id') => HavocConflictingWrites(s, s', id, id')
+      case HavocConflictingWriteReadStep(id, id') => HavocConflictingWriteRead(s, s', id, id')
+    }
+  }
+
+  predicate NextInternal(s: Variables, s': Variables)
+  {
+    exists step :: NextInternalStep(s, s', step)
+  }
+
+  predicate Crash(s: Variables, s': Variables)
+  {
+    s' == Variables(map[], map[], map[], map[], s.contents)
+  }
+}
